Hashmap/HashMap.lean
@@ -5,8 +5,9 @@ Authors: Leonardo de Moura, Mario Carneiro, Markus Himmel
 -/
 import Hashmap.AssocList.Map
 import Hashmap.LawfulHashable
+import Std.Data.Array.Lemmas
 
-namespace Lean
+namespace MyLean
 
 namespace HashMap.Imp
 
@@ -15,41 +16,53 @@ def Buckets (α : Type u) [BEq α] (β : α → Type v) :=
 
 namespace Buckets
 
-def update [BEq α] (b : Buckets α β) (i : USize) (h : i.toNat < b.1.size) (l : AssocListMap α β) : Buckets α β :=
-  ⟨b.1.uset i l h, by simpa using b.2⟩
+def update [BEq α] (b : Buckets α β) (i : Fin b.1.size) (l : AssocListMap α β) : Buckets α β :=
+  ⟨b.1.set i l, by simpa using b.2⟩
 
 @[simp]
-theorem update_size [BEq α] {b : Buckets α β} {i : USize} {h : i.toNat < b.1.size} {l : AssocListMap α β} :
-    (b.update i h l).1.size = b.1.size := by simp [update]
+theorem update_size [BEq α] {b : Buckets α β} (i : Fin b.1.size) {l : AssocListMap α β} :
+    (b.update i l).1.size = b.1.size := by simp [update]
 
--- Todo: this is insane
-macro_rules
-| `(tactic| get_elem_tactic_trivial) => `(tactic| simpa)
+theorem update_get [BEq α] {b : Buckets α β} {i : Fin b.1.size} {l : AssocListMap α β}
+    {j : Fin (b.update i l).1.size}:
+    (b.update i l).1[j] = if (i : Nat) = j then l else b.1[j] := by
+  simp [update]
+  rw [Array.get_set]
 
-theorem update_get [BEq α] {b : Buckets α β} {i : USize} {h : i.toNat < b.1.size} {l : AssocListMap α β}
-    {j : USize} {hj : j.toNat < b.1.size} :
-    (b.update i h l).1[j] = if i = j then l else b.1[j] := by
-  sorry -- Meh
+structure BucketWFAt [BEq α] [Hashable α] (l : AssocListMap α β)
+    (size i : Nat) : Prop where
+  hash_valid [LawfulHashable α] : ∀ a, l.contains a → (hash a % size).toNat = i
 
-structure BucketWFAt [BEq α] [Hashable α] [LawfulHashable α] (l : AssocListMap α β)
-    (size : Nat) (index : USize) : Prop where
-  hash_valid : ∀ a, l.contains a → (hash a % size).toNat = i
+theorem BucketWFAt_nil [BEq α] [Hashable α] {size i : Nat} :
+    BucketWFAt (AssocListMap.nil : AssocListMap α β) size i where
+  hash_valid a h := by simp at h
+
+theorem BucketWFAt_erase [BEq α] [EquivBEq α] [Hashable α] {l : AssocListMap α β} {k : α} {size i : Nat} :
+    BucketWFAt l size i → BucketWFAt (l.erase k) size i :=
+  fun ⟨h⟩ => ⟨fun a h' => h a <| l.contains_of_contains_erase h'⟩
+
+theorem BucketWFAt_insert [BEq α] [EquivBEq α] [Hashable α] {l : AssocListMap α β} {k : α} {v : β k} {size i : Nat}
+    (h : (hash k % size).toNat = i) : BucketWFAt l size i → BucketWFAt (l.insert k v) size i := by
+  refine fun ⟨h⟩ => ⟨fun a h' => ?_⟩
+  rw [l.contains_insert, Bool.or_eq_true] at h'
+  rcases h' with (h'|h')
+  · rwa [← hash_eq_of_beq h']
+  · exact h _ h'
 
 structure WF [BEq α] [Hashable α] [LawfulHashable α] (b : Buckets α β) : Prop where
-  bucket_wf : ∀ (i : USize) (h : i.toNat < b.1.size), BucketWFAt b.1[i] b.1.size i
+  bucket_wf : ∀ (i : Fin b.1.size), BucketWFAt b.1[i] b.1.size i
 
-theorem WF_update [BEq α] [Hashable α] [LawfulHashable α] {b : Buckets α β} {i : USize} {h : i.toNat < b.1.size}
-    {l : AssocListMap α β} : b.WF → BucketWFAt l b.1.size i → (b.update i h l).WF := by
-  refine fun ⟨h₁⟩ h₂ => ⟨fun j hj => ?_⟩
+theorem WF_update [BEq α] [Hashable α] [LawfulHashable α] {b : Buckets α β} {i : Fin b.1.size}
+    {l : AssocListMap α β} : b.WF → BucketWFAt l b.1.size i → (b.update i l).WF := by
+  refine fun ⟨h₁⟩ h₂ => ⟨fun j => ?_⟩
   rw [update_get]
-  by_cases h' : i = j
+  by_cases h' : i.1 = j
   · simpa [h'] using h₂
   · simp [h']
-    apply h₁ j
-  · simpa using hj
+    apply h₁ (Fin.cast (by simp) j)
 
 end Buckets
 
 end HashMap.Imp
 
-end Lean
+end MyLean
